src/tlogic/TemporalLogic.v
@@ -2,7 +2,6 @@ From stdpp Require Import coPset gmap namespaces.
 From sflib Require Import sflib.
 From Fairness Require Import PCM IProp IPM.
 From Fairness Require Import IndexedInvariants LogicSyntaxHOAS.
-(* From Fairness Require Import IndexedInvariants LogicSyntaxHOAS PCMForSyntax PCMEmbed. *)
 (* From Fairness Require Import ISim. *)
 From iris Require Import bi.big_op.
 From iris Require base_logic.lib.invariants.
@@ -10,8 +9,6 @@ From iris Require base_logic.lib.invariants.
 Local Notation index := nat.
 
 Section TLOGIC.
-
-  Local Notation index := nat.
 
   Section TYPE.
 
@@ -39,6 +36,9 @@ Section TLOGIC.
 
     Context `{As : forall formula : Type, Type}.
 
+    Definition _formula : index -> Type :=
+      @Syntax._formula type (@Typ) As.
+
     Definition formula : index -> Type :=
       @Syntax.formula type (@Typ) As.
 
@@ -49,11 +49,10 @@ Section TLOGIC.
     Context `{As : forall formula : Type, Type}.
 
     Context `{Σ : GRA.t}.
-    Context `{interp_atoms_0 : As Empty_set -> iProp}.
-    Context `{interp_atoms : forall (n : index), As (@formula As n) -> iProp}.
+    Context `{interp_atoms : forall (n : index), As (@_formula As n) -> iProp}.
 
     Definition formula_sem : forall n, formula n -> iProp :=
-      @Syntax.to_semantics type (@Typ) As Σ interp_atoms_0 interp_atoms.
+      @Syntax.to_semantics type (@Typ) As Σ interp_atoms.
 
   End INTERP.
 
@@ -67,12 +66,18 @@ Module Atoms.
     (* | own {A : Atom} (a : A.(T)) *)
     | owni (i : positive) (p : @Syntax.t type (@Typ) (@t form) form)
     (* | syn_inv_auth_l (ps : list (prod positive form)) *)
+    (* (* for invariant system *) *)
+    (* | owni (i : positive) (p : t) *)
+    (* | syn_inv_auth_l (ps : list (prod positive t)) *)
+    (* (* Non strictly positive occurrence *) *)
+    (* (* | own_inv_auth (ps : gmap positive t) *) *)
     .
 
   End ATOMS.
 
   Section INTERP.
 
+    Local Notation _Formula := (@_formula (@t)).
     Local Notation Formula := (@formula (@t)).
 
     Context `{Σ : PCM.GRA.t}.
@@ -83,21 +88,34 @@ Module Atoms.
     (* Context `{@PCM.GRA.inG (PCM.URA.pointwise index PCM.CoPset.t) Σ}. *)
     (* Context `{@PCM.GRA.inG (PCM.URA.pointwise index PCM.Gset.t) Σ}. *)
 
-    (* Definition to_semantics_0 (a : @t Σ Empty_set) : iProp := *)
-    Definition to_semantics_0 (a : @t Empty_set) : iProp :=
+    Definition to_semantics n (a : @t (_Formula n)) : iProp :=
       match a with
-      (* | @own _ _ A r => A.(interp) r *)
-      | owni i p => @OwnI Σ Formula _ O i p
+      | owni i p => @OwnI Σ Formula _ n i p
       (* | syn_inv_auth_l ps => @inv_auth Σ Formulas _ n (list_to_map ps) *)
       end.
 
-    (* Definition to_semantics n (a : @t Σ (Formula n)) : iProp := *)
-    Definition to_semantics n (a : @t (Formula n)) : iProp :=
-      match a with
-      (* | @own _ _ A r => A.(interp) r *)
-      | owni i p => @OwnI Σ Formula _ (S n) i p
-      (* | syn_inv_auth_l ps => @inv_auth Σ Formulas _ n (list_to_map ps) *)
-      end.
+    (* Definition to_semantics n (a : @t (Formula n)) : iProp := *)
+    (*   match a with *)
+    (*   | owni i p => @OwnI Σ Formula _ (S n) i p *)
+    (*   (* | syn_inv_auth_l ps => @inv_auth Σ Formulas _ n (list_to_map ps) *) *)
+    (*   end. *)
+
+
+    (* (* Definition to_semantics_0 (a : @t Σ Empty_set) : iProp := *) *)
+    (* Definition to_semantics_0 (a : @t Empty_set) : iProp := *)
+    (*   match a with *)
+    (*   (* | @own _ _ A r => A.(interp) r *) *)
+    (*   | owni i p => @OwnI Σ Formula _ O i p *)
+    (*   (* | syn_inv_auth_l ps => @inv_auth Σ Formulas _ n (list_to_map ps) *) *)
+    (*   end. *)
+
+    (* (* Definition to_semantics n (a : @t Σ (Formula n)) : iProp := *) *)
+    (* Definition to_semantics n (a : @t (Formula n)) : iProp := *)
+    (*   match a with *)
+    (*   (* | @own _ _ A r => A.(interp) r *) *)
+    (*   | owni i p => @OwnI Σ Formula _ (S n) i p *)
+    (*   (* | syn_inv_auth_l ps => @inv_auth Σ Formulas _ n (list_to_map ps) *) *)
+    (*   end. *)
 
   End INTERP.
 
@@ -115,13 +133,16 @@ Section TL.
 
   Context `{@PCM.GRA.inG (IInvSetRA Formula) Σ}.
 
-  Local Notation AtomSem0 := (@Atoms.to_semantics_0 Σ _).
-  Local Notation AtomSem := (@Atoms.to_semantics Σ _).
-  Local Notation SynSem := (@formula_sem (@Atoms.t) Σ AtomSem0 AtomSem).
+  (* Local Notation AtomSem0 := (@Atoms.to_semantics_0 Σ _). *)
+  Definition AtomSem := (@Atoms.to_semantics Σ _).
+  Definition SynSem n : Formula n -> iProp := (@formula_sem (@Atoms.t) Σ AtomSem n).
+  (* Local Notation SynSem := (@formula_sem (@Atoms.t) Σ AtomSem0 AtomSem). *)
   (* Local Notation SynSem := (@formula_sem (@Atoms.t Σ) Σ AtomSem0 AtomSem). *)
 
   Global Instance SynIISet : @IInvSet Σ Formula :=
-    (@Syntax.IISet _ _ _ Σ AtomSem0 AtomSem).
+    (@Syntax.IISet _ _ _ Σ AtomSem).
+  (* Global Instance SynIISet : @IInvSet Σ Formula := *)
+  (*   (@Syntax.IISet _ _ _ Σ AtomSem0 AtomSem). *)
 
   (* Global Instance IIIn (i : index) (p : Formula i) : @IInvIn Σ Formula SynIISet i (SynSem i p) := *)
   (*   @Syntax.IIIn _ _ _ Σ AtomSem0 AtomSem i p. *)
@@ -131,15 +152,65 @@ End TL.
 Section TEST.
 
   Context `{Σ : GRA.t}.
+  Context `{@PCM.GRA.inG (IInvSetRA Formula) Σ}.
 
-  Check (Syntax.atom (Atoms.owni xH (Syntax.ex formulaT (fun (p : Formula 2) => Syntax.pure (p = Syntax.empty)) : Formula 3))) : Formula 3.
-  Check (Syntax.atom (Atoms.owni xH (Syntax.ex formulaT (fun p => Syntax.pure (p = Syntax.empty))))) : Formula 3.
+  Definition test0 := ((Syntax.atom (Atoms.owni xH (Syntax.ex formulaT (fun (p : Formula 2) => Syntax.pure (p = Syntax.empty)) : Formula 3))) : Formula 3).
+  Let test1 := (Syntax.atom (Atoms.owni xH (Syntax.ex formulaT (fun (p : Formula 2) => Syntax.pure (p = Syntax.empty)) : Formula 3))) : Formula 3.
+  Let test2 := (Syntax.atom (Atoms.owni xH (Syntax.ex formulaT (fun p => Syntax.pure (p = Syntax.empty))))) : Formula 3.
+
   Fail Check (Syntax.atom (Atoms.owni xH (Syntax.ex formulaT (fun (p : Formula 2) => Syntax.pure (p = Syntax.empty)) : Formula 2))) : Formula 3.
   Fail Check (Syntax.atom (Atoms.owni xH (Syntax.ex formulaT (fun (p : Formula 1) => Syntax.pure (p = Syntax.empty))))) : Formula 3.
   Fail Check (Syntax.atom (Atoms.owni xH (Syntax.ex formulaT (fun (p : Formula 0) => Syntax.pure (p = Syntax.empty))))) : Formula 3.
 
+  Goal (SynSem _ test1) = OwnI 3 xH (Syntax.ex formulaT (fun (p : Formula 2) => Syntax.pure (p = Syntax.empty))).
+  Proof.
+    ss.
+  Qed.
+
+  Goal (SynSem _ (Syntax.sepconj test1 test2 : Formula 3)) =
+         ((OwnI 3 xH (Syntax.ex formulaT (fun (p : Formula 2) => Syntax.pure (p = Syntax.empty)))) ∗ (OwnI 3 xH (Syntax.ex formulaT (fun (p : Formula 2) => Syntax.pure (p = Syntax.empty)))))%I.
+  Proof.
+    subst test1 test2. setoid_rewrite red_sem_sepconj. ss.
+  Qed.
+
 End TEST.
 
+
+(*   Section GMAP. *)
+
+(*     Context `{Σ : GRA.t}. *)
+(*     Context `{As : (type -> Type) -> Type}. *)
+
+(*     Local Notation typing := (@Typ As). *)
+(*     Local Notation Formulas := (fun (i : index) => @t (typing i) (As (typing i))). *)
+
+(*     Context `{interp_atoms : forall (n : index), As (typing n) -> iProp}. *)
+
+(*     (* Maybe we can make Syntax as an instance of bi. *) *)
+(*     Definition star_gmap *)
+(*                (n : index) (I : typing (S n) (pgmapT formulaT)) *)
+(*                (f : positive -> Formulas n -> Formulas n) *)
+(*       : Formulas n := *)
+(*       fold_right (fun hd tl => @sepconj (typing n) (As (typing n)) (uncurry f hd) tl) empty (map_to_list I). *)
+
+
+(*     Local Notation Sem := (fun i p => @to_semantics Σ As interp_atoms i p). *)
+
+(*     Lemma star_gmap_iProp *)
+(*           n I f *)
+(*       : *)
+(*       Sem n (star_gmap n I f) = *)
+(*         ([∗ map] i ↦ p ∈ I, Sem n (f i p))%I. *)
+(*     Proof. *)
+(*       ss. unfold big_opM. rewrite seal_eq. unfold big_op.big_opM_def. *)
+(*       unfold star_gmap. ss. remember (map_to_list I) as L. *)
+(*       clear HeqL I. induction L. *)
+(*       { ss. apply to_semantics_empty. } *)
+(*       ss. rewrite to_semantics_red_sepconj. rewrite IHL. f_equal. *)
+(*       destruct a. ss. *)
+(*     Qed. *)
+
+(*   End GMAP. *)
 
 
 (* Old *)
@@ -276,344 +347,3 @@ End TEST.
 (*   Qed. *)
 
 (* End WSAT. *)
-
-(* TODO *)
-(* Section FUPD. *)
-
-  
-
-(* End FUPD. *)
-
-
-(*   Context `{Σ : GRA.t}. *)
-(*   Context `{Vars : index -> Type}. *)
-(*   Context `{Invs : @IInvSet Σ Vars}. *)
-(*   (* Context `{Invs : @InvSet Σ (Vars n)}. *) *)
-(*   Context `{@GRA.inG (index ==> CoPset.t)%ra Σ}. *)
-(*   Context `{@GRA.inG (index ==> Gset.t)%ra Σ}. *)
-(*   Context `{@GRA.inG (IInvSetRA Vars) Σ}. *)
-
-(*   Variable n : index. *)
-
-(*   Local Notation Var := (Vars n). *)
-
-(*   Definition inv (N : namespace) P := *)
-(*     (∃ p, ∃ i, ⌜prop n p = P⌝ ∧ ⌜i ∈ (↑N : coPset)⌝ ∧ OwnI n i p)%I. *)
-
-(*   Definition FUpd (A : iProp) (E1 E2 : coPset) (P : iProp) : iProp := *)
-(*     (* A ∗ wsat (prop:=prop n) n ∗ OwnE n E1 -∗ #=> (A ∗ wsat (prop:=prop n) n ∗ OwnE n E2 ∗ P). *) *)
-(*     A ∗ wsat n ∗ OwnE n E1 -∗ #=> (A ∗ wsat n ∗ OwnE n E2 ∗ P). *)
-
-
-(*   Section INDEXED_INVSET. *)
-
-(*     Context `{Σ : GRA.t}. *)
-(*     Context `{T : Type}. *)
-(*     Context `{TSem : T -> Type}. *)
-
-(*     Local Notation typing := (@Syntax.Typ T TSem (@t T)). *)
-(*     Local Notation As := (fun (i : index) => @t T (typing i)). *)
-(*     Local Notation Formulas := (fun (i : index) => @Syntax.t T (typing i) (As i)). *)
-
-(*     Context `{@GRA.inG (IInvSetRA Formulas) Σ}. *)
-
-(*     Global Instance IISet : @IInvSet Σ As := *)
-(*       {| prop := @to_semantics Σ T TSem _ |}. *)
-
-(*   End INDEXED_INVSET. *)
-
-(*   Section TEST. *)
-
-(*     Context `{Σ : GRA.t}. *)
-
-(*     Local Notation T := Base.t. *)
-(*     Local Notation TSem := Base.sem. *)
-
-(*     Local Notation typing := (@Syntax.Typ T TSem (@t T)). *)
-(*     Local Notation Formulas := (fun (i : index) => @Syntax.t T (typing i) (@t T (typing i))). *)
-
-(*     Context `{@GRA.inG (IInvSetRA Formulas) Σ}. *)
-
-(*     Global Instance testIISet : IInvSet Formulas := *)
-(*       @Syntax.IISet Σ T TSem (@t T) IISet. *)
-
-(*     Import Base. *)
-(*     Import Syntax. *)
-
-(*     Definition wsat n : Formulas (S n) := *)
-(*       ex formulaT (fun p => ex (baseT positiveT) (fun i => sepconj (lift p) (lift (atom (owni n i p))))). *)
-
-(*     Lemma wsat_test1 : *)
-(*       prop 3 (wsat 2) = *)
-(*         (∃ (p : Formulas 2) (i : positive), (prop 2 p) ∗ (OwnI 2 i p))%I. *)
-(*     Proof. *)
-(*       ss. *)
-(*     Qed. *)
-
-(*   End TEST. *)
-
-
-(*   Section TEST. *)
-
-(*     Import Syntax. *)
-
-(*     Context `{TSem : T -> Type}. *)
-
-(*     Local Notation t := Atom.t. *)
-
-
-(*     Local Notation typing := (@Syntax.Typ T TSem t). *)
-(*     Local Notation Formulas := (fun (i : index) => @Syntax.t T (typing i) (t (typing i))). *)
-
-(*     Definition test1 : Formulas 3 := *)
-(*       atom (owni 4 xH (atom (owni 2 xH empty))). *)
-
-(*     Definition test_OwnI (n : index) (i : positive) (p : Formulas n) : t (typing n) := *)
-(*       @owni (typing n) n i p. *)
-
-(*     (* Set Printing All. *) *)
-
-(*   End TEST. *)
-
-(* Module Atom. *)
-
-(*   Section ATOMS. *)
-
-(*     (* Context `{T : Type}. *) *)
-
-(*     Context `{σ : list PCMForSyntax.URA.t}. *)
-
-(*     (* TODO: more atoms *) *)
-
-(*     (* Atom do not interpret arguments. *) *)
-(*     Inductive t {Typ : Syntax.type -> Type} : Type := *)
-(*     | own {M : PCMForSyntax.URA.t} {IN : In M σ} (r : M) *)
-(*     (* | own {M : PCMForSyntax.URA.t} {IN : PCMForSyntax.GRA.inG M σ} (r : M) *) *)
-(*     | owne (E : coPset) *)
-(*     | ownd (D : gset positive) *)
-(*     | owni (i : positive) (p : @Syntax.t Typ (@t Typ)) *)
-(*     | syn_inv_auth_l (ps : list (prod positive (@Syntax.t Typ (@t Typ)))) *)
-(*     (* Non strictly positive occurrence *) *)
-(*     (* | own_inv_auth (ps : gmap positive (@Syntax.t Typ (@t Typ))) *) *)
-(*     . *)
-
-(*   End ATOMS. *)
-
-(*   Section INTERP. *)
-
-(*     Context `{σ : list PCMForSyntax.URA.t}. *)
-(*     (* Local Notation σ := (PCMForSyntax.GRA.of_list _σ). *) *)
-(*     (* Context `{σ : PCMForSyntax.GRA.t}. *) *)
-(*     Context `{Σ : PCM.GRA.t}. *)
-(*     (* Context `{T : Type}. *) *)
-(*     (* Context `{TSem : T -> Type}. *) *)
-(*     Context `{SUB : forall M, In M σ -> PCM.GRA.inG (to_LURA M) Σ}. *)
-
-(*     (* This is too strong. *) *)
-(*     (* Context `{SUB : forall (M : URA.t), PCMForSyntax.GRA.inG M σ -> PCM.GRA.inG (to_LURA M) Σ}. *) *)
-
-(*     Local Notation typing := (@Syntax.Typ (@t σ)). *)
-(*     Local Notation Formulas := (fun (i : index) => @Syntax.t (typing i) (@t σ (typing i))). *)
-(*     (* Local Notation typing := (@Syntax.Typ T TSem (@t T)). *) *)
-(*     (* Local Notation Formulas := (fun (i : index) => @Syntax.t T (typing i) (@t T (typing i))). *) *)
-
-(*     Context `{@PCM.GRA.inG (IInvSetRA Formulas) Σ}. *)
-(*     Context `{@PCM.GRA.inG (PCM.URA.pointwise index PCM.CoPset.t) Σ}. *)
-(*     Context `{@PCM.GRA.inG (PCM.URA.pointwise index PCM.Gset.t) Σ}. *)
-
-(*     Definition to_semantics (n : index) (a : @t σ (typing n)) : iProp := *)
-(*       match a with *)
-(*       | @own _ _ M IN r => @OwnM Σ (to_LURA M) (SUB M IN) r *)
-(*       | owne E => OwnE n E *)
-(*       | ownd D => OwnD n D *)
-(*       | owni i p => @OwnI Σ Formulas _ n i p *)
-(*       | syn_inv_auth_l ps => @inv_auth Σ Formulas _ n (list_to_map ps) *)
-(*       end. *)
-
-(*     (* Definition to_semantics (n : index) (a : @t T (typing n)) : iProp := *) *)
-(*     (*   match a with *) *)
-(*     (*   | owne E => OwnE n E *) *)
-(*     (*   | ownd D => OwnD n D *) *)
-(*     (*   | owni i p => @OwnI Σ Formulas _ n i p *) *)
-(*     (*   | syn_inv_auth_l ps => @inv_auth Σ Formulas _ n (list_to_map ps) *) *)
-(*     (*   end. *) *)
-
-(*   End INTERP. *)
-
-(* End Atom. *)
-
-
-  (* Definition inv (N : namespace) P := *)
-  (*   (∃ p, ∃ i, ⌜prop n p = P⌝ ∧ ⌜i ∈ (↑N : coPset)⌝ ∧ OwnI n i p)%I. *)
-
-  (* Definition FUpd (A : iProp) (E1 E2 : coPset) (P : iProp) : iProp := *)
-  (*   A ∗ wsat n ∗ OwnE n E1 -∗ #=> (A ∗ wsat n ∗ OwnE n E2 ∗ P). *)
-
-
-
-(*   Context `{T : Type}. *)
-(*     Context `{TSem : T -> Type}. *)
-
-(*     (* Atom should not interpret arguments. *) *)
-(*     Inductive As (V : @type T -> Type) : Type := *)
-(*       | owni (p : V formulaT) *)
-(*     . *)
-(*     (* Inductive As (V : @type T -> Type) : Type := *) *)
-(*     (*   | owni (i : index) (p : @t T V (As V)) *) *)
-(*     (* . *) *)
-
-(*     Definition typing (i : index) : @type T -> Type := *)
-(*       @Typ T TSem As i. *)
-
-(*     (* Definition ttt1 : As (typing 2) := owni (typing 2) 0 (ex formulaT (fun s => pure (s = empty))). *) *)
-(*     (* Compute ttt1. *) *)
-(*     Definition ttt1 : As (typing 2) := owni (typing 2) (ex formulaT (fun s => pure (s = empty))). *)
-(*     Compute ttt1. *)
-(*     Goal typing 2 formulaT = @t T (typing 1) (As (typing 1)). *)
-(*     Proof. *)
-(*       ss. *)
-(*     Qed. *)
-
-(*     Definition inv (i : index) (p : typing i formulaT) : *)
-(*       @t T (typing i) (As (typing i)) := *)
-(*       atom (owni _ p). *)
-(*     (* Definition inv (n i : index) (p : @t T (typing i) (As (typing i))) : *) *)
-(*     (*   @t T (typing i) (As (typing i)) := *) *)
-(*     (*   atom (owni _ n p). *) *)
-(*     Definition wsat (i : index) : *)
-(*       @t T (typing i) (As (typing i)) := *)
-(*       ex formulaT (fun (p : typing i formulaT) => sepconj (lift p) (inv i p)). *)
-
-(*     (* Definition inv0 (n i : index) (p : @t T (typing 2) (As (typing 2))) : *) *)
-(*     (*   @t T (typing 3) (As (typing 2)) := *) *)
-(*     (*   atom (owni _ n p). *) *)
-
-(*     (* (* Definition of As enforces that  *) *)
-(*     (*    p should have the same typing level for itself and its atom  *) *)
-(*     (*  *) *) *)
-(*     (* Fail Definition inv1 (n : index) (p : @t T (typing 2) (As (typing 3))) : *) *)
-(*     (*   @t T (typing 2) (As (typing 3)) := *) *)
-(*     (*   atom (owni _ n p). *) *)
-
-(*     (* Definition inv2 q := *) *)
-(*     (*   inv 0 3 (atom (owni _ 1 (atom (owni _ 2 q)))). *) *)
-
-(*     (* Fail Definition inv2' q := *) *)
-(*     (*   inv 0 3 (atom (owni _ 1 (atom (owni (typing 2) 2 q)))). *) *)
-
-(*     (* Set Printing All. *) *)
-
-(*     (* Definition inv (N : namespace) P := *) *)
-(*     (*   (∃ p, ∃ i, ⌜prop p = P⌝ ∧ ⌜i ∈ (↑N : coPset)⌝ ∧ OwnI n i p)%I. *) *)
-
-
-
-
-
-(*   Section TEST. *)
-
-(*     Context `{A : Type}. *)
-
-(*     Variant tBase := | tBool | tNat. *)
-(*     Definition tBase_sem (b : tBase) : Type := *)
-(*       match b with | tBool => bool | tNat => nat end. *)
-
-(*     Let Var := @Var tBase tBase_sem A. *)
-
-(*     Compute Var 3 formulaT. *)
-
-(*     (* Goal Var 3 formulaT = @t _ (Var 2) A formulaT. *) *)
-(*     Goal Var 3 formulaT = @t _ (Var 2) A. *)
-(*     Proof. ss. Qed. *)
-
-(*     Definition syn_bad i := @t tBase (@Var i) A. *)
-(*     Notation syn i := (@t tBase (@Var i) A). *)
-
-(*     (* Definition form1 : @syn 2 formulaT := *) *)
-(*     Definition form1 : @syn 2 := *)
-(*       @ex _ _ _ (baseT tBool) (fun b => empty). *)
-
-(*     (* Goal (syn 1 formulaT) = (Var 2 formulaT). *) *)
-(*     Goal (syn 1) = (Var 2 formulaT). *)
-(*     Proof. ss. Qed. *)
-
-(*     (* Definition form2 : @syn 2 formulaT := *) *)
-(*       (* @ex _ _ _ formulaT (fun (s : Var 2 formulaT) => and (var _ s) (var _ s)). *) *)
-(*     Definition form2 : @syn 2 := *)
-(*       @ex _ _ _ formulaT (fun (s : Var 2 formulaT) => pure (s = impl empty empty)). *)
-
-(*     (* Definition form3 : @syn 2 formulaT := *) *)
-(*     (*   @ex _ _ _ formulaT (fun (s : @t tBase (Var 1) A formulaT) => and (var _ s) (var _ s)). *) *)
-(*     Definition form3 : @syn 2 := *)
-(*       @ex _ _ _ formulaT (fun (s : @t tBase (Var 1) A) => pure (s = impl empty empty)). *)
-
-(*     (* Definition form4 : @syn 2 formulaT := *) *)
-(*     (*   @ex _ _ _ formulaT (fun (s : @syn 1 formulaT) => and (var _ s) (var _ s)). *) *)
-(*     Definition form4 : @syn 2 := *)
-(*       @ex _ _ _ formulaT (fun (s : @syn 1) => pure (s = impl empty empty)). *)
-
-(*     (* Definition form5 : @syn 2 formulaT := *) *)
-(*     (*   @ex _ _ _ formulaT (fun (s : @syn 1 formulaT) => pure (s = wand empty empty)). *) *)
-(*     Definition form5 : @syn 2 := *)
-(*       @ex _ _ _ formulaT (fun (s : @syn 1) => pure (s = wand empty empty)). *)
-
-(*   End TEST. *)
-
-(* Section TEST. *)
-
-(*     Context `{T : Type}. *)
-(*     Context `{TSem : T -> Type}. *)
-
-(*     (* Atom should not interpret arguments. *) *)
-(*     Inductive As (V : @type T -> Type) : Type := *)
-(*       | owni (p : V formulaT) *)
-(*     . *)
-(*     (* Inductive As (V : @type T -> Type) : Type := *) *)
-(*     (*   | owni (i : index) (p : @t T V (As V)) *) *)
-(*     (* . *) *)
-
-(*     Definition typing (i : index) : @type T -> Type := *)
-(*       @Typ T TSem As i. *)
-
-(*     (* Definition ttt1 : As (typing 2) := owni (typing 2) 0 (ex formulaT (fun s => pure (s = empty))). *) *)
-(*     (* Compute ttt1. *) *)
-(*     Definition ttt1 : As (typing 2) := owni (typing 2) (ex formulaT (fun s => pure (s = empty))). *)
-(*     Compute ttt1. *)
-(*     Goal typing 2 formulaT = @t T (typing 1) (As (typing 1)). *)
-(*     Proof. *)
-(*       ss. *)
-(*     Qed. *)
-
-(*     Definition inv (i : index) (p : typing i formulaT) : *)
-(*       @t T (typing i) (As (typing i)) := *)
-(*       atom (owni _ p). *)
-(*     (* Definition inv (n i : index) (p : @t T (typing i) (As (typing i))) : *) *)
-(*     (*   @t T (typing i) (As (typing i)) := *) *)
-(*     (*   atom (owni _ n p). *) *)
-(*     Definition wsat (i : index) : *)
-(*       @t T (typing i) (As (typing i)) := *)
-(*       ex formulaT (fun (p : typing i formulaT) => sepconj (lift p) (inv i p)). *)
-
-(*     (* Definition inv0 (n i : index) (p : @t T (typing 2) (As (typing 2))) : *) *)
-(*     (*   @t T (typing 3) (As (typing 2)) := *) *)
-(*     (*   atom (owni _ n p). *) *)
-
-(*     (* (* Definition of As enforces that  *) *)
-(*     (*    p should have the same typing level for itself and its atom  *) *)
-(*     (*  *) *) *)
-(*     (* Fail Definition inv1 (n : index) (p : @t T (typing 2) (As (typing 3))) : *) *)
-(*     (*   @t T (typing 2) (As (typing 3)) := *) *)
-(*     (*   atom (owni _ n p). *) *)
-
-(*     (* Definition inv2 q := *) *)
-(*     (*   inv 0 3 (atom (owni _ 1 (atom (owni _ 2 q)))). *) *)
-
-(*     (* Fail Definition inv2' q := *) *)
-(*     (*   inv 0 3 (atom (owni _ 1 (atom (owni (typing 2) 2 q)))). *) *)
-
-(*     (* Set Printing All. *) *)
-
-(*     (* Definition inv (N : namespace) P := *) *)
-(*     (*   (∃ p, ∃ i, ⌜prop p = P⌝ ∧ ⌜i ∈ (↑N : coPset)⌝ ∧ OwnI n i p)%I. *) *)
-
-(* End TEST. *)
